HOL_To_IMP_Minus/Refinements/HOL_To_IMP_Minus_TSAT_To_IS.thy
@@ -1,8 +1,70 @@
 theory HOL_To_IMP_Minus_TSAT_To_IS
   imports
-    HOL_To_IMP_Minus_Arithmetics
-    Karp21.TSAT_To_IS_List
+    HOL_To_IMP_Minus_Lists
+    (* Karp21.TSAT_To_IS_List *)
 begin
+
+context HOL_To_HOL_Nat
+begin
+
+definition "map_rpair_acc y \<equiv> map_acc (rpair y)"
+lemmas map_rpair_acc_eq = map_acc_eq[of "rpair y" for y, folded map_rpair_acc_def]
+function_compile_nat map_rpair_acc_eq
+
+fun case_prod_map_rpair where "case_prod_map_rpair (x, xs) = map (rpair x) xs"
+
+case_of_simps case_prod_map_rpair_eq[unfolded map_eq_map_acc_nil,
+  folded map_rpair_acc_def] : case_prod_map_rpair.simps
+function_compile_nat case_prod_map_rpair_eq
+
+definition "map_case_prod_map_rpair_acc \<equiv> map_acc case_prod_map_rpair"
+lemmas map_case_prod_map_rpair_acc_eq = map_acc_eq[of "case_prod_map_rpair",
+  folded map_case_prod_map_rpair_acc_def]
+function_compile_nat map_case_prod_map_rpair_acc_eq
+
+end
+
+context HOL_Nat_To_IMP_Minus
+begin
+
+lemmas map_rpair_acc_nat_eq = HTHN.map_rpair_acc_nat_eq_unfolded[simplified case_list_nat_def]
+compile_nat map_rpair_acc_nat_eq
+HOL_To_IMP_Minus_correct HOL_To_HOL_Nat.map_rpair_acc_nat
+  supply Rel_nat_destruct_Cons[Rel_nat]
+  apply (tactic \<open>HM.correct_if_IMP_tailcall_correct_tac HT.get_IMP_def @{context} 1\<close>)
+  by (induction "HTHN.rpair y :: 'b \<Rightarrow> _" _ _ arbitrary: s rule: HOL_To_HOL_Nat.map_acc.induct)
+  (tactic \<open>HT.start_run_finish_case_tac HT.get_IMP_def HT.get_imp_minus_correct
+    HB.get_HOL_eqs @{context} 1\<close>)+
+
+lemmas case_prod_map_rpair_nat_eq = HTHN.case_prod_map_rpair_nat_eq_unfolded[simplified case_prod_nat_def]
+compile_nat case_prod_map_rpair_nat_eq
+HOL_To_IMP_Minus_correct HOL_To_HOL_Nat.case_prod_map_rpair_nat
+  supply Rel_nat_destruct_Pair[Rel_nat] by (cook mode = induction)
+
+lemmas map_case_prod_map_rpair_acc_nat_eq =
+  HTHN.map_case_prod_map_rpair_acc_nat_eq_unfolded[simplified case_list_nat_def]
+compile_nat map_case_prod_map_rpair_acc_nat_eq
+HOL_To_IMP_Minus_correct HOL_To_HOL_Nat.map_case_prod_map_rpair_acc_nat
+  supply Rel_nat_destruct_Cons[Rel_nat]
+  apply (tactic \<open>HM.correct_if_IMP_tailcall_correct_tac HT.get_IMP_def @{context} 1\<close>)
+  by (induction "HTHN.case_prod_map_rpair :: ('a \<times> 'b list) \<Rightarrow> _" _ _ arbitrary: s
+    rule: HOL_To_HOL_Nat.map_acc.induct)
+  (tactic \<open>HT.start_run_finish_case_tac HT.get_IMP_def HT.get_imp_minus_correct
+    HB.get_HOL_eqs @{context} 1\<close>)+
+
+end
+
+    (* let
+      p1 = enumerate 0 F;
+      p2 = map (\<lambda>(xsa, xsb). map (\<lambda>x. (x, xsa)) xsb) p1;
+      p3 = map (\<lambda>xs. List.product xs xs) p2;
+      p4 = map (\<lambda>xs. filter (\<lambda>((a, _), (b, _)). a \<noteq> b) xs) p3;
+      p5 = concat p4;
+      p6 = map (\<lambda>(a, b). [a, b]) p5
+    in p6"
+ *)
+
+
 
 (*TODO: compiled and verify reduction here + move tairec funds from
 Tail_Rec_Funs into corresponding locale *)
